feat: remove Substring.Raw instance

Lemmas/Basic.lean
@@ -18,17 +18,6 @@ class Stream.Remaining (σ : Type) where
   /--  natural number measure of remaining input -/
   remaining : σ -> Nat
 
-/-- enables usage of Substring.Raw as σ -/
-class Stream.ValidPosition (σ : Type) [Stream.Remaining σ] where
-  /-- condition for σ -/
-  valid : σ -> Prop
-  /- is valid for remaining input -/
-  validOfRemaining (it : σ) (h : 0 < Stream.Remaining.remaining it) : valid it
-
-/-- defines streams where Stream.ValidPosition is not necessary -/
-class Stream.AllValid (σ : Type) [Stream.Remaining σ] [Stream.ValidPosition σ] where
-  valid : ∀ (it : σ), Stream.ValidPosition.valid it
-
 /-- remaining input of ```rem``` is less than remaining input of ```it``` -/
 def Stream.decrementsRemaining [Stream.Remaining σ] (it rem : σ)
     := Stream.Remaining.remaining rem < Stream.Remaining.remaining it
@@ -41,24 +30,21 @@ def Stream.notIncrementsRemaining [Stream.Remaining σ] (it rem : σ)
   with the following steps
 
 * save current position
-* aplly a parser that respects the position
+* apply a parser that respects the position
 * reset to the saved position
  -/
-class Stream.RespectsPosition (σ τ : Type) [Parser.Stream σ τ] [Stream.Remaining σ] [Stream.ValidPosition σ] where
+class Stream.RespectsPosition (σ τ : Type) [Parser.Stream σ τ] [Stream.Remaining σ]  where
   /-- respectsPosition relation -/
   r : σ → σ → Prop
   /-- no input is consumed if the position is reset after applying a respectful parser -/
-  setPosition_of_getPosition_eq (s1 s2 : σ) (p : Position σ) :
-    Stream.ValidPosition.valid s1
-    → Stream.getPosition s1 = p
-    → r s1 s2
-    → Stream.setPosition s2 p = s1
+  setPosition_of_getPosition_eq (s1 s2 : σ) (p : Position σ)
+      : Stream.getPosition s1 = p  → r s1 s2 → Stream.setPosition s2 p = s1
     /-- respectsPosition is a equivalence relation -/
   isEquivalence : Equivalence r
 
  /-- `Stream.RespectsPosition` relation -/
 abbrev Stream.respectsPosition [Parser.Stream σ τ] [Stream.Remaining σ]
-    [Stream.ValidPosition σ] [Stream.RespectsPosition σ τ] (s1 s2 : σ) : Prop :=
+    [Stream.RespectsPosition σ τ] (s1 s2 : σ) : Prop :=
   Stream.RespectsPosition.r τ s1 s2
 
 /-- a parser consumes no input if the corresponding streams are equal -/
@@ -66,25 +52,24 @@ def consumesNoInput (σ τ : Type) [Parser.Stream σ τ] (p : SimpleParser σ τ
     := ∀ it, (match (p it) with | .ok rem _ => rem | .error rem _ => rem) = it
 
 /-- a parser respects positions if the corresponding streams respect positions -/
-def respectsPosition (σ τ : Type) [Parser.Stream σ τ] [Stream.Remaining σ] [Stream.ValidPosition σ]
+def respectsPosition (σ τ : Type) [Parser.Stream σ τ] [Stream.Remaining σ]
   [Stream.RespectsPosition σ τ] (p : SimpleParser σ τ α)
-  := ∀ it rem, Stream.ValidPosition.valid it
-                → (match (p it) with | .ok rem _ => rem | .error rem _ => rem) = rem
+  := ∀ it rem, (match (p it) with | .ok rem _ => rem | .error rem _ => rem) = rem
                 → Stream.respectsPosition it rem
 
 /-- a parser not increments input on success if the corresponding streams not increment input  -/
 def notIncrementsRemainingOnSuccess (σ τ : Type) [Parser.Stream σ τ] [Stream.Remaining σ]
-  [Stream.ValidPosition σ] (p : SimpleParser σ τ α)
-  := ∀ it rem a, Stream.ValidPosition.valid it → p it = .ok rem a → Stream.notIncrementsRemaining it rem
+   (p : SimpleParser σ τ α)
+  := ∀ it rem a, p it = .ok rem a → Stream.notIncrementsRemaining it rem
 
 /-- a parser decrements input on success if the corresponding streams decrement input  -/
 def decrementsRemainingOnSuccess (σ τ : Type) [Parser.Stream σ τ] [Stream.Remaining σ]
-  [Stream.ValidPosition σ] (p : SimpleParser σ τ α)
-  := ∀ it rem a, Stream.ValidPosition.valid it → p it = .ok rem a → Stream.decrementsRemaining it rem
+   (p : SimpleParser σ τ α)
+  := ∀ it rem a, p it = .ok rem a → Stream.decrementsRemaining it rem
 
 /-- Defines the postcondition of Std.Stream.next? on a non empty stream with class Stream.RespectsPosition
  -/
-class Stream.Next?OnInput (σ τ : Type) [Parser.Stream σ τ] [Stream.Remaining σ] [Stream.ValidPosition σ]
+class Stream.Next?OnInput (σ τ : Type) [Parser.Stream σ τ] [Stream.Remaining σ]
   [Stream.RespectsPosition σ τ] where
   cond (it : σ) : 0 < Stream.Remaining.remaining it
                   → ∃ rem t, Std.Stream.next? it = some (t, rem)
@@ -93,14 +78,12 @@ class Stream.Next?OnInput (σ τ : Type) [Parser.Stream σ τ] [Stream.Remaining
 
 /-- Defines the postcondition of Std.Stream.next? on an empty stream -/
 class Stream.Next?OnEndOfInput (σ τ : Type) [Parser.Stream σ τ] [Stream.Remaining σ]
-  [Stream.ValidPosition σ] where
-  cond (it : σ) : Stream.ValidPosition.valid it
-                  → (0 = Stream.Remaining.remaining it)
-                  → Std.Stream.next? it = none
+   where
+  cond (it : σ) : (0 = Stream.Remaining.remaining it) → Std.Stream.next? it = none
 
 /-- Defines a precondition for Stream.setPosition, so that Parser.setPosition gives a valid result
  -/
-class Stream.SetPositionPrecondition (σ τ : Type) [Parser.Stream σ τ] [Stream.Remaining σ] [Stream.ValidPosition σ]
+class Stream.SetPositionPrecondition (σ τ : Type) [Parser.Stream σ τ] [Stream.Remaining σ]
   [Stream.RespectsPosition σ τ] where
   /-- precondition for Stream.setPosition -/
   cond : σ →  Stream.Position σ → Prop
@@ -110,15 +93,11 @@ class Stream.SetPositionPrecondition (σ τ : Type) [Parser.Stream σ τ] [Strea
                           ∧ pos = Parser.Stream.getPosition rem
                           ∧ Stream.respectsPosition it rem
   /-- Stream.getPosition gives the ```cond``` precondition -/
-  of_getPosition s1 s2 p :
-    Stream.ValidPosition.valid s1
-    → Stream.getPosition s1 = p
-    → Stream.respectsPosition s1 s2
-    → cond s2 p
+  of_getPosition s1 s2 p : Stream.getPosition s1 = p → Stream.respectsPosition s1 s2 → cond s2 p
 
 /-- example with decrementsRemainingOnSuccess to prove termination -/
-def foldr'  (σ τ : Type) [Parser.Stream σ τ] [Stream.Remaining σ] [Stream.ValidPosition σ]
-  [Stream.AllValid σ] (f : α → β → β) (p : SimpleParser σ τ α) (q : SimpleParser σ τ β)
+def foldr'  (σ τ : Type) [Parser.Stream σ τ] [Stream.Remaining σ]
+  (f : α → β → β) (p : SimpleParser σ τ α) (q : SimpleParser σ τ β)
   (h : decrementsRemainingOnSuccess σ τ p)
     : SimpleParser σ τ β := foldrAux
 where
@@ -129,7 +108,7 @@ where
     | .ok s' x =>
       have : Stream.Remaining.remaining s' < Stream.Remaining.remaining s := by
         simp [decrementsRemainingOnSuccess] at h
-        exact h s s' x (Stream.AllValid.valid s) (by grind)
+        exact h s s' x (by grind)
       foldrAux s' >>= fun
       | .ok s'' y => return .ok s'' (f x y)
       | .error s'' e => return .error s'' e
