Lemmas.lean
@@ -3,5 +3,4 @@ module
 public import Lemmas.Basic
 public import Lemmas.Lemmas
 public import Lemmas.String.Instances
-public import Lemmas.Substring.Instances
 public import Lemmas.List.Instances
